$$
% 极限
\newcommand{\liml}{\lim\limits}
\newcommand{\ulim}{\overline\lim\limits_{n\to\infty}}
\newcommand{\dlim}{\underline\lim\limits_{n\to\infty}}
% 注意这里的 d 是 down, 而不是 displaystyle

\newcommand{\xlim}{\lim\limits_{x\to x_0}}
\newcommand{\nlim}{\lim\limits_{n\to\infty}}
\newcommand{\clim}[1]{\lim\limits_{#1\to\infty}}

% 并集
\newcommand{\incup}{\bigcup_{i=1}^n}
\newcommand{\nocup}{\bigcup_{n=1}^\infty}
\newcommand{\iocup}{\bigcup_{i=1}^\infty}

% 交集
\newcommand{\incap}{\bigcap_{i=1}^n}
\newcommand{\nocap}{\bigcap_{n=1}^\infty}
\newcommand{\iocap}{\bigcap_{i=1}^\infty}

\begin{align}
P\pqty{\nocap \bigcup_{i = n}^\infty A_i}
&= P\pqty{\nlim \bigcup_{i = n}^\infty A_i}
= \nlim P\pqty{\bigcup_{i = n}^\infty A_i}
\\
&= 1 - \nlim P\pqty{\bigcap_{i = n}^\infty A_i^C}
= 1 - \nlim \prod_{i = n}^\infty P(A_i^C)
\\
&= 1 - \nlim \prod_{i = n}^\infty (1 - P(A_i))
\ge  1 - \nlim \prod_{i = n}^\infty \mathrm{e}^{-P(A_i)}
\\
&= 1 - \nlim \exp\pqty{- \sum_{i = n}^\infty P(A_i)}
= 0.
\end{align}
$$

从而得证.