由 $ N(s + t) - N(s) $ 和 $ N(t) - N(0) $ 同分布, 即得增量平稳性.
$$
\newcommand{\e}{\mathrm{e}}
\begin{align}
% \lim_{\Delta t \to 0+}
% \dfrac{
% 	P\Bqty{N(t + \Delta t) - N(t) = k}
% }{\Delta t}
% &= \lim_{\Delta t \to 0+}
% \dfrac{
% 	(\lambda \Delta t)^k
% }{k! \Delta t} \e^{-\lambda \Delta t}
P\Bqty{N(t + \Delta t) - N(t) = k}
% \\
% =& \dfrac{
% 	(\lambda \Delta t)^k
% }{k!} \e^{-\lambda \Delta t}
% \\
= \begin{cases}
	\e^{-\lambda \Delta t}
	= 1 - \lambda \Delta t + \omicron(\Delta t),
	& k = 0, \\
	\lambda \Delta t \e^{-\lambda \Delta t}
	= \lambda \Delta t + \omicron(\Delta t),
	& k = 1, \\
	\dfrac{
		(\lambda \Delta t)^k
	}{k!} \e^{-\lambda \Delta t}
	= \omicron(\Delta t), & k > 1.
\end{cases}
\end{align}
$$

从而得证.