由增量平稳性, 记
$$
\newcommand{\e}{\mathrm{e}}
\begin{align}
P_n(t) &= P\Bqty{N(s + t) - N(s) = n} \\
&= P\Bqty{N(t) = n}.
\end{align}
$$
当 $ n = 0 $ 时, 由增量独立性知
$$
\begin{align}
P_0\pqty{t + h} &= P\Bqty{N(t + h) = 0}
\\
&= P\Bqty{N(t) = 0, N(t + h) - N(t) = 0}
\\
&= P\Bqty{N(t) = 0} P\Bqty{N(t + h) - N(t) = 0}
\\
&= P_0(t) P_0(h).
\end{align}
$$
由微分性质知
$$
\begin{align}
P_0(h) &= P\Bqty{N(t + h) - N(h) = 0}
\\
&= 1 - \lambda h - \omicron(h).
\end{align}
$$
代入导数定义得
$$
\begin{align}
P'_0(t) &= \lim_{h \to 0} \dfrac{
	P_0(t + h) - P_0(t)
}{h} \\
&= \lim_{h \to 0} \dfrac{
	- \lambda h - \omicron(h)
}{h} P_0(t)
\\
&= -\lambda P_0(t).
\end{align}
$$
代入初值 $ P_0(0) = P\Bqty{N(0) = 0} = 1 $ 得 $ P_0(t) = \e^{-\lambda t} $.

当 $ n > 0 $ 时, 由微分性质知
$$
\begin{align}
P_n(t + h) &= P\Bqty{N(t + h) = n}
\\
% &= P\Bqty{N(t) = n} P\Bqty{N(h) = 0}
% + P\Bqty{N(t) = n-1} P\Bqty{N(h) = 1}
% \\
&= P_n(t) (1 - \lambda h - \omicron(h)) +
\\
&\quad\; P_{n - 1}(t) (\lambda h + \omicron(h)) + \omicron(h).
\end{align}
$$
代入导数定义得
$$
\begin{align}
P'_n(t) &= \lim_{h \to 0} \dfrac{
	P_n(t + h) - P_n(t)
}{h} \\
&= -\lambda P_n(t) + \lambda P_{n-1}(t).
\end{align}
$$
考虑初值 $ P_n(0) = P\Bqty{N(0) = n} = 0 $, 于是由数学归纳法得
$$
P_n(t) = \dfrac{(\lambda t)^n}{n!} \e^{-\lambda t}.
$$