记
$$
\newcommand{\nlim}{\lim\limits_{n\to\infty}}

\begin{align}
A &= \Bqty{\omega \mid N(\infty) = \infty},
\\
B &= \Bqty{\omega \mid \nlim \dfrac{S_n}{n} = \mu},
\\
C &= \Bqty{\omega \mid \lim_{t \to \infty} \dfrac{S_{N(t)}}{N(t)} = \mu},
\\
D &= \Bqty{\omega \mid \lim_{t \to \infty} \dfrac{N(t)}{t} = \dfrac{1}{\mu}}.
\end{align}
$$
则 $ P(A) = P(B) = 1 $, 于是
$$
\begin{align}
P(AB) &= P(A) + P(B) - P(A + B)
\\
&= 2 - P(A + B) = 1.
\end{align}
$$
而 $ AB \subseteq C \Rightarrow P(C) = 1 $.

由 $ S_{N(t)} \le t < S_{N(t) + 1} $,
$$
\begin{align}
\mu &= \lim_{t \to \infty} \dfrac{S_{N(t)}}{N(t)}
\le \lim_{t \to \infty} \dfrac{t}{N(t)}
\le \lim_{t \to \infty} \dfrac{S_{N(t) + 1}}{N(t) + 1} \cdot \dfrac{N(t) + 1}{N(t)} = \mu.
\end{align}
$$
即 $ C \subseteq D $, 于是 $ P(D) = 1 $. 证毕.