令 $ I_n = I_\Bqty{T \ge n} $, 即
$$
% 求和
\newcommand{\dsum}{\displaystyle\sum}
\newcommand{\csum}[1]{\dsum_{#1=1}^\infty}
\newcommand{\nsum}{\csum{n}}
\newcommand{\ksum}{\csum{k}}
\newcommand{\nosum}{\dsum_{n=0}^\infty}
\newcommand{\insum}{\dsum_{i=1}^n}
\newcommand{\knsum}{\dsum_{k=1}^n}

\newcommand{\ssto}[3]{#1_1 #3 #1_2 #3 \cdots #3 #1_{#2}}
\newcommand{\soneto}[2]{\ssto{#1}{#2}{,}}

I_n = \begin{cases}
	1, & T \ge n, \\
	0, & T < n.
\end{cases}
$$
则 $ \dsum_{n = 1}^T X_n = \nsum X_n I_n $, 且
$$
\begin{align}
\Bqty{I_n = 0} &= \Bqty{T < n}
= \bigcup_{k = 1}^{n - 1} \Bqty{T = k},
\end{align}
$$
于是 $ \Bqty{I_n = 0} $ 及其补集 $ \Bqty{I_n = 1} $ 仅依赖于 $ \soneto{X}{n-1} $,

因此 $ I_n $ 与 $ X_n $ 独立, 于是
$$
\begin{align}
E\pqty{\sum_{n = 1}^T X_n}
&= E\pqty{\nsum X_n I_n}
= \nsum E(X_n) E(I_n)
\\
&= E(X) \nsum E(I_n)
= E(X) \nsum P\Bqty{T \ge n}
= E(X) E(T).
\end{align}
$$
证毕.