令 $ G(x) = 1 - F(x) = P\Bqty{W(t) > x} $,

则 $ G(0) = 1 $, 并且 $ G(x) $ 是单调不增的右连续函数.

代入定理 2.3.2, 得
$$
\newcommand{\e}{\mathrm{e}}
\begin{align}
G(x) &= G(x + t) - \int_0^t G(x) \dd{G(u)}
\\
&= G(x + t) - G(x)G(t) + G(x),
\end{align}
$$
于是有
$$
G(x + t) = G(x) G(t),
$$
两端对 $x$ 求导, 得
$$
\begin{align}
G'_x(x) G(t) &= G'_x(x + t) = G'_t(x + t),
\end{align}
$$
令 $ x= 0 $, $ \lambda = -G'_x(0) $, 则
$$
\begin{align}
G'_t(t) &= -\lambda G(t),
\\
G(t) &= \e^{-\lambda t},
\\
F(x) &= 1 - \e^{-\lambda x}.
\end{align}
$$
于是由定理 2.2.1 知 $ \Bqty{N(t), t \ge 0} $ 为 Poisson 过程.