$$
P\Bqty{W(t) > x} = \int_0^{+\infty} P\Bqty{W(t) > x \mid X_1 = s} \dd{F(s)}.
$$

1. 当 $ s > t + x $ 时, $ P\Bqty{W(t) > x \mid X_1 = s} = 1 $.
2. 当 $ t \le s < s + t $ 时, $ P\Bqty{W(t) > x \mid X_1 = s} = 0 $.
3. 当 $ s < t $ 时,

$$
\begin{align}
&\hspace{1.3em}
P\Bqty{W(t) > x \mid X_1 = s}
\\
&= P\Bqty{S_{N(t) + 1} - t > x \mid X_1 = s}
\\
&= P\Bqty{ \left.
	\sum_{j = 2}^{N(t) + 1} X_j + s - t > x
	\ \right|\ X_1 = s
} \\
&= \sum_{m = 1}^\infty P\Bqty{ \left.
	\sum_{j = 2}^{m + 1} X_j + s - t > x , N(t) = m
	\ \right|\ X_1 = s
} \\
&= \sum_{m = 1}^\infty P\Bqty{ \left.
	\sum_{j = 2}^{m + 1} X_j + s - t > x,
	S_m \le t < S_{m + 1}
	\ \right|\ X_1 = s
} \\
&= \sum_{m = 1}^\infty P\Bqty{ \left.
	\sum_{j = 2}^{m + 1} X_j + s - t > x,
	\sum_{j = 2}^m X_j \le t - s < \sum_{j = 2}^{m + 1} X_j
	\ \right|\ X_1 = s
} \\
&= \sum_{m = 1}^\infty P\Bqty{
	\sum_{j = 2}^{m + 1} X_j + s - t > x,
	\sum_{j = 2}^m X_j \le t - s < \sum_{j = 2}^{m + 1} X_j
} \\
&= \sum_{m = 1}^\infty P\Bqty{
	S_m + s - t > x, S_{m - 1} \le t - s < S_m
} \\
&= \sum_{m = 1}^\infty P\Bqty{
	S_m + s - t > x, N(t - s) = m - 1
} \\
&= P\Bqty{S_{N(t - s)} - (t - s) > x}
\\
&= P\Bqty{W(t - s) > x}.
\end{align}
$$

代入以上三式即得所求证公式.