由定理 2.2.1, 只需证 $ \Bqty{X_n, n \ge 1} $ 独立同分布 $ E(\lambda) $.

再由定理 2.2.3 的证明过程, 只需证对于 $ G(x) = 1 - F(x) $, 有 $ G(x + s) = G(x) G(s) $.

由题意, 注意到
$$
P\Bqty{
	X_1 \ge s \mid N(s + x) = 1
} + P\Bqty{
	X_1 \ge x \mid N(s + x) = 1
} = \dfrac{x}{s + x} + \dfrac{s}{s + x} = 1.
$$
利用条件概率与全概率的公式, 得
$$
\newcommand{\dint}{\displaystyle\int}

\begin{align}
P\Bqty{
	X_1 \ge s \mid N(s + x = 1)
} &= \dfrac{
	P\Bqty{X_1 \le s, X_1 \le s + x < X_1 + X_2}
}{
	P\Bqty{X_1 \le s + x < X_1 + X_2}
} \\
&= \dfrac{
	\dint_0^s [1 - F(s + x - u)] \dd{F(u)}
}{
	\dint_0^{s + x} [1 - F(s + x - u)] \dd{F(u)}
},
\end{align}
$$
代入前式并化简, 得
$$
% \begin{align}
% \int_0^x [1 - F(s + x - u)] \dd{F(u)} +
% \int_0^s [1 - F(s + x - u)] \dd{F(u)} =
% \int_0^{s + x} [1 - F(s + x - u)] \dd{F(u)}
% \end{align}
\int_0^s [1 - F(s + x - u)] \dd{F(u)}
= \int_x^{x + s} [1 - F(s + x - u)] \dd{F(u)},
\\
F(s) + F(x) - F(s) F(x) = F(x + s),
\\
G(x + s) = G(x) G(s).
$$
从而得证.