记 $ P_n(t) = P\Bqty{N(s + t) - N(s) = n} $,

**1.**	当 $ n = 0 $ 时,
$$
\begin{align}
P_0(t + h) &= P\Bqty{N(s + t + h) - N(s) = 0}
\\
&= P\Bqty{N(s + t) - N(s) = 0}
P\Bqty{N(s + t + h) - N(s + t) = 0}
\\
&= P_0(t) [1 - \lambda(t) h - \omicron(h)],
\end{align}
$$
代入导数定义, 得
$$
\begin{align}
P'_0(t) &= \lim_{h \to 0} \dfrac{P_0(t + h) - P_0(t)}{h}
\\
&= \lim_{h \to 0} \dfrac{-\lambda (t) h - \omicron(h)}{h} P_0(t)
\\
&= -\lambda(t) P_0(t).
\end{align}
$$
代入初值 $ P_0(0) = 1 $, 得 $ P_0(t) = \mathrm{e}^{m(s) - m(s + t)} $.

**2.**	当 $ n \ge 1 $ 时,
$$
\begin{align}
P_n(t + h) &= P\Bqty{N(s + t + h) - N(s) = n}
\\
&= P_n(t) [1 - \lambda(t) h - \omicron(h)] +
P_{n-1}(t) (\lambda h + \omicron(h)) + \omicron(h),
\end{align}
$$
代入导数定义, 得
$$
\begin{align}
P'_n(t) &= \lim_{h \to 0} \dfrac{
	P_n(t + h) - P_n(t)
}{h}
\\
&= -\lambda(t) P_n(t) + \lambda(t) P_{n-1}(t).
\end{align}
$$
考虑初值 $ P_n(0) = 0 $, 于是由数学归纳法得
$$
P{\Bqty{N(s + t) - N(s) = n}}
= \dfrac{
	[m(s + t) - m(s)]^n
}{n!} \mathrm{e}^{m(s) - m(s + t)}.
$$
证毕.