$$
\newcommand{\bm}[1]{\boldsymbol{#1}}

\begin{align}
p_{ij}^{(m + n)}
&=
P\Bqty{
	X_{m + n} = j \mid X_0 = i
} \\
&= \sum_{k \in S} P\Bqty{
	X_m = k, X_{m + n} = j \mid X_0 = i
}
\\
&= \sum_{k \in S} P\Bqty{
	X_m = k \mid X_0 = i
} P\Bqty{
	X_{m + n} = j \mid X_0 = i, X_m = k
} \\
&= \sum_{k \in S} p_{ik}^{(m)} p_{kj}^{(n)}.
\end{align}
$$

写成向量形式即为 $ \bm P^{(m + n)} = \bm P^{(m)} \bm P^{(n)} $. 且有
$$
\begin{align}
\bm P^{(n)} &= \bm P^{(n-1)} \bm P^{(1)} 
= \pqty{\bm P^{(1)}}^n
= \bm P^n.
\end{align}
$$
从而得证.