由 $ i \to j $, 得 $ \exist m > 0: p_{ij}^{m} > 0 $, 于是
$$
% 求和
\newcommand{\dsum}{\displaystyle\sum}
\newcommand{\csum}[1]{\dsum_{#1=1}^\infty}
\newcommand{\nsum}{\csum{n}}
\newcommand{\ksum}{\csum{k}}
\newcommand{\nosum}{\dsum_{n=0}^\infty}
\newcommand{\insum}{\dsum_{i=1}^n}
\newcommand{\knsum}{\dsum_{k=1}^n}



\begin{align}
p_{ij}^{(m + n)} &= \sum_{k \in S} p_{ik}^{(m)} p_{kj}^{(n)} \ge p_{ij}^{(m)} p_{jj}^{(n)},
\\
\nsum p_{ij}^{(n)} &\ge
\nsum p_{ij}^{(m + n)}
\ge p_{ij}^{(m)} \nsum p_{jj}^{(n)}
= \infty.
\end{align}
$$
第二点由定义即得. 证毕.