对于状态 $ i $,
$$
% 求和
\newcommand{\dsum}{\displaystyle\sum}
\newcommand{\csum}[1]{\dsum_{#1=1}^\infty}
\newcommand{\nsum}{\csum{n}}
\newcommand{\ksum}{\csum{k}}
\newcommand{\nosum}{\dsum_{n=0}^\infty}
\newcommand{\insum}{\dsum_{i=1}^n}
\newcommand{\knsum}{\dsum_{k=1}^n}

\begin{align}
p_{ii}^{(2n-1)} &= 0,
\\
p_{ii}^{(2n)} &= \binom{2n}{n} p^n q^n.
\end{align}
$$
考虑母函数
$$
\begin{align}
P_{ii}(z) &= \nosum \binom{2n}{n} p^n q^n z^{2n}
\\
&= \nosum \dfrac{
	2^{2n} (-1)^n
}{n!} \pqty{-\dfrac{1}{2}}
\pqty{-\dfrac{3}{2}} \cdots
\pqty{-\dfrac{2n-1}{2}}
(pqz^2)^n
\\
&= (1 - 4pqz^2)^{-\tfrac{1}{2}},
\end{align}
$$
其中最后一步可参考[高数笔记](https://sleepcloudmx.github.io/Math/分析/高数/image/高数上/13.png). 从而有
$$
\begin{align}
\nosum p_{ii}^{(n)} &= P_{ii}(1)
= \lim_{z \to 1-} P_{ii}(z) = \begin{cases}
	\infty, & p = \frac{1}{2}, \\
	(1 - 4pqz^2)^{-\frac{1}{2}}, & p \ne \frac{1}{2}.
\end{cases}
\end{align}
$$
于是当且仅当 $ p = \dfrac{1}{2} $ 时 $ i $ 是常返的, 从而该等价类常返. 证毕.