**1.**	证明 $ \forall i, j \in S: 0 \le g_{ij} \le f_{ij} $.

对于 $ f_{ij} $, 考虑
$$
% 求和
\newcommand{\dsum}{\displaystyle\sum}
\newcommand{\csum}[1]{\dsum_{#1=1}^\infty}
\newcommand{\nsum}{\csum{n}}
\newcommand{\ksum}{\csum{k}}
\newcommand{\nosum}{\dsum_{n=0}^\infty}
\newcommand{\insum}{\dsum_{i=1}^n}
\newcommand{\knsum}{\dsum_{k=1}^n}

% 并集
\newcommand{\incup}{\bigcup_{i=1}^n}
\newcommand{\ncup}{\bigcup_{n=1}^\infty}
\newcommand{\icup}{\bigcup_{i=1}^\infty}

% 交集
\newcommand{\incap}{\bigcap_{i=1}^n}
\newcommand{\ncap}{\bigcap_{n=1}^\infty}
\newcommand{\icap}{\bigcap_{i=1}^\infty}

\newcommand{\RA}{\Rightarrow}
\newcommand{\rla}{\leftrightarrow}


\begin{align}
\Bqty{T_{ij} \le \infty, X_0 = i}
&= \ncup \Bqty{T_{ij} = n, X_0 = i}
\\
&= \ncup \Bqty{X_0 = i, X_l \ne j, 0 < l < n, X_n = j}
\\
&= \ncup \Bqty{X_0 = i, X_n = j},
\end{align}
$$
对于 $ g_{ij} $, 考虑
$$
\begin{align}
\Bqty{S_1(j) = \infty, X_0 = i}
&= \bigcap_{m=1}^\infty \bigcup_{n=m}^\infty\Bqty{X_0 = i, X_n = j}
\\
&\subset \ncup \Bqty{X_0 = i, X_n = j},
\end{align}
$$
于是有
$$
\begin{align}
0 \le g_{ij} &= P\Bqty{S_1(j) = \infty \mid X_0 = i}
\\
&\le P\Bqty{T_{ij} < \infty \mid X_0 = i} = f_{ij}.
\end{align}
$$
**2.**	证明 $ f_{ji} = 1 $.
$$
i \to j \RA \exist m > 0: p_{ij}^{(m)} > 0,
$$

$$
\forall h \in S: \Bqty{
	X_0 = i, S_1(h) = +\infty
} = \bigcup_{k \in S} \Bqty{
	X_0 = i, X_m = k, S_{m + 1}(h) = +\infty
},
$$

于是
$$
g_{ih} = \sum_{k \in S} p_{ik}^{(m)} P\Bqty{
	S_{m + 1}(h) = +\infty \mid X_0 = i, X_m = k
} = \sum_{k \in S} p_{ik}^{(m)} g_{kh}.
$$
由 $ i $ 常返, 即 $ f_{ii} = 1 $, 得
$$
\begin{align}
0 &= 1 - f_{ii}
= \sum_{k \in S} p_{ik}^{(m)} - \sum_{k \in S} p_{ik}^{(m)} g_{ki}
\\
&= \sum_{k \in S} p_{ik}^{(m)} (1 - g_{ki}) \ge p_{ij}^{(m)} (1 - g_{ji}) \ge 0,
\end{align}
$$
从而 $ 1 = g_{ji} \le f_{ji} \le 1 $, 即 $ f_{ji} = 1 $, 且 $ j \to i $.

**3.**	证明 $ j $ 常返.

由 $ i \rla j $, 设 $ p_{ji}^{(r)} = \alpha > 0, p_{ij}^{(s)} = \beta > 0 $, 则
$$
\forall n \ge 0:
p_{jj}^{(r + n + s)} \ge p_{ji}^{(r)} p_{ii}^{(n)} p_{ij}^{s} = \alpha \beta p_{ii}^{(n)}.
$$
于是
$$
\nsum p_{jj}^{(n)} \ge \alpha \beta \nsum p_{jj}^{(n)} = +\infty.
$$
即 $ j $ 常返. 证毕.