**1.**	由定理 3.4.2 及上述引理 1 即得.

**2.1**	当 $ n = 1 $ 时, 由引理 2 即得.

**2.2**	当 $ n > 1 $ 时, 由 C-K 方程,
$$
\newcommand{\bm}[1]{\boldsymbol{#1}}

\begin{align}
\bm P^n &= \bm P^{n-1} \bm P = \begin{bmatrix}
	\bm P_C^{n-1} & \bm 0 \\
	\bm R_{n-1} & \bm Q_T^{n-1}
\end{bmatrix} \begin{bmatrix}
	\bm P_C & \bm 0 \\
	\bm R & \bm Q_T
\end{bmatrix}
\\
&= \begin{bmatrix}
	\bm P_C^{n-1} \bm P_C & \bm 0 \\
	\bm R_{n-1} \bm P_C + \bm Q_T^{n-1} \bm R & \bm Q_T^{n-1} \bm Q_T
\end{bmatrix}
\\
&= \begin{bmatrix}
	\bm P_C^n & \bm 0 \\
	\bm R_n & \bm Q_T^n
\end{bmatrix}.
\end{align}
$$
从而得证.

**3.**	由定理 3.3.2 推论 1 即得.

证毕.