1. 绝对期望

$$
\begin{align}
E\vqty{X_n} &= \sum_{k=0}^n E\vqty{
	\pqty{
		f(Z_k) - E[f(Z_k) \mid Y_0, \cdots, Y_{k-1}]
	} a_k(Y_0, \cdots, Y_{k-1})
} \\
&\le \sum_{k=0}^n 2 E\vqty{f(Z_k)} A_k < \infty,
\end{align}
$$

2. 条件期望

记
$$
B_k = \pqty{
	f(Z_k) - E[f(Z_k) \mid Y_0, \cdots, Y_{k-1}]
} a_k(Y_0, \cdots, Y_{k-1}),
$$
则
$$
\begin{align}
&\hspace{1.3em} E(B_k \mid Y_0, \cdots, Y_{k-1})
\\
&= a_k(Y_0, \cdots, Y_{k-1}) E[f(Z_k) \mid Y_0, \cdots, Y_{k-1}] -
\\
&\hspace{1.3em} a_k(Y_0, \cdots, Y_{k-1}) E[E[f(Z_k) \mid Y_0, \cdots, Y_{k-1}] \mid Y_0, \cdots, Y_{k-1}]
 =0,
\end{align}
$$
从而
$$
E(X_{n + 1} \mid Y_0, \cdots, Y_n)
= E(X_n \mid Y_0, \cdots, Y_n) + E(B_{n + 1} \mid Y_0, \cdots, Y_n) = X_n.
$$
从而为鞅.