**1.**	证明 $ E\pqty{X_n I_\Bqty{T > n, S = k}} $ 对于 $n$ 是单调递增函数.

对于固定的 $ k \le n $, 注意到 $ I_\Bqty{T > n} $ 仅依赖于 $ Y_0, \cdots, Y_n $, 于是有
$$
\begin{align}
E\pqty{
	X_{n + 1} I_\Bqty{T > n, S = k}
} &= E\bqty{
	E\pqty{
		X_{n + 1} I_\Bqty{T > n, S = k}
	} \mid Y_0, \cdots, Y_n
} \\
&= E\bqty{
	E\pqty{
		X_{n + 1}
	} \mid Y_0, \cdots, Y_n
} I_\Bqty{T > n, S = k}
\\
&\ge E\bqty{
	X_n I_\Bqty{T > n, S = k}
},
\end{align}
$$
**2.**	证明 $ E\pqty{X_{T \and n} I_\Bqty{S = k}} $ 对于 $n$ 是单调递增函数.
$$
\begin{align}
E\pqty{
	X_{T \and n} I_\Bqty{S = k}
} &= E\pqty{
	X_T I_\Bqty{T \le n, S = k}
} + E\pqty{
	X_n I_\Bqty{T > n, S = k}
} \\
&\le E\pqty{
	X_T I_\Bqty{T \le n, S = k}
} + E\pqty{
	X_{n + 1} I_\Bqty{T > n, S = k}
} \\
&= E\pqty{
	X_{T \and (n + 1)} I_\Bqty{T \le n, S = k}
} + E\pqty{
	X_{T \and (n + 1)} I_\Bqty{T > n, S = k}
} \\
&= E\pqty{
	X_{T \and (n + 1)} I_\Bqty{S = k}
},
\end{align}
$$
**3.**	证明 $ EX_S \le EX_T $.

由第二点与假设 $ S \le T $, 有
$$
\begin{align}
EX_S &= E\pqty{
	\sum_{k = 0}^N X_S I_\Bqty{S = k}
} = \sum_{k = 0}^N E\pqty{
	X_S I_\Bqty{S = k}
} \\
&\le \sum_{k = 0}^N E\pqty{
	X_T I_\Bqty{S = k}
} = E\pqty{
	X_T \sum_{k = 0}^N I_\Bqty{S = k}
} = EX_T,
\end{align}
$$
证毕.