记圆为 $ (z - a)(\overline{z} - \overline{a}) = R^2 $, 则有
$$
\begin{align}
\overline{(z, z_1, z_2, z_3)}
&= \overline{
	(z - a, z_1 - a, z_2 - a, z_3 - a)
} \\
&= \pqty{
	\overline z - \overline a,
	\dfrac{R^2}{z_1 - a},
	\dfrac{R^2}{z_2 - a},
	\dfrac{R^2}{z_3 - a}
} \\
&= \pqty{
	\dfrac{R^2}{\overline z - \overline a},
	z_1 - a, z_2 - a, z_3  -a
} \\
&= \pqty{
	\dfrac{R^2}{\overline z - \overline a} + a,
	z_1, z_2, z_3
}
\end{align}
$$
由此可得出 $ z^* $ 的表达式:
$$
\begin{align}
z^* &= \dfrac{R^2}{\overline z - \overline a} + a
\\
R^2 &= (z^* - a)(\overline z - \overline a)
\\
&= \vqty{z^* - a} \cdot \vqty{z - a}
\end{align}
$$
又由于
$$
\dfrac{z^* - a}{z - a} = \dfrac{R^2}{\vqty{z - a}^2} > 0
$$
所以 $ z $ 与 $ z^* $ 在 $a$ 的同侧, 且关于圆 $C$ 反演.